Working on generating terms, test plus for nat

tools/src/main/scala/lam2gu/DeBruijnEncoder.scala
@@ -1,0 +1,133 @@
+package lam2gu
+
+import lam2gu.ASTs.{ConcreteSyntax => CS, DeBruijnSyntax => DS}
+
+object DeBruijnEncoder {
+  def encode(expression: CS.Expression): DS.Expression =
+    encSub(expression, Map.empty, Map.empty)
+
+  case class UnknownIdentifier(name: String)
+      extends IllegalArgumentException(s"Unknown identifier $name")
+
+  type Subst = Map[String, Int]
+
+  // TODO rewrite this to use some kind of reader/state monad
+  def encSub(
+      expresssion: CS.Expression,
+      exprSubst: Subst,
+      typSubst: Subst
+  ): DS.Expression =
+    expresssion match {
+      case CS.LamVar(name) => DS.LamVar(exprSubst.deref(name))
+      case CS.FixVar(name) => DS.FixVar(exprSubst.deref(name))
+      case CS.ConstructorApp(name, types, arg) =>
+        DS.ConstructorApp(
+          name,
+          types.map(encSubT(_, typSubst)),
+          encSub(arg, exprSubst, typSubst)
+        )
+      case CS.VUnit => DS.VUnit
+      case CS.VTuple(fst, snd) =>
+        DS.VTuple(
+          encSub(fst, exprSubst, typSubst),
+          encSub(snd, exprSubst, typSubst)
+        )
+      case CS.Fst(e) =>
+        DS.Fst(encSub(e, exprSubst, typSubst))
+      case CS.Snd(e) =>
+        DS.Snd(encSub(e, exprSubst, typSubst))
+      case CS.Lambda(arg, argType, body) =>
+        DS.Lambda(
+          (),
+          encSubT(argType, typSubst),
+          encSub(body, exprSubst.enterBinder(arg), typSubst)
+        )
+      case CS.Application(fun, arg) =>
+        DS.Application(
+          encSub(fun, exprSubst, typSubst),
+          encSub(arg, exprSubst, typSubst)
+        )
+      case CS.TypeLambda(arg, body) =>
+        DS.TypeLambda((), encSub(body, exprSubst, typSubst.enterBinder(arg)))
+      case CS.TypeApplication(e, arg) =>
+        DS.TypeApplication(
+          encSub(e, exprSubst, typSubst),
+          encSubT(arg, typSubst)
+        )
+      case CS.Fix(selfName, selfType, body) =>
+        DS.Fix(
+          (),
+          encSubT(selfType, typSubst),
+          encSub(body, exprSubst.enterBinder(selfName), typSubst)
+        )
+      case CS.CaseOf(e, clauses) =>
+        DS.CaseOf(
+          encSub(e, exprSubst, typSubst),
+          clauses.map {
+            case CS.Clause(pattern, body) =>
+              val (pat, eP, tP) = encPat(pattern, exprSubst, typSubst)
+              val encBody = encSub(body, eP, tP)
+              DS.Clause(pat, encBody)
+          }
+        )
+      case CS.Let(name, bound, body) =>
+        DS.Let(
+          (),
+          encSub(bound, exprSubst, typSubst),
+          encSub(body, exprSubst.enterBinder(name), typSubst)
+        )
+    }
+
+  def encPat(
+      pattern: CS.Pattern,
+      exprSubst: Subst,
+      typSubst: Subst
+  ): (DS.Pattern, Subst, Subst) =
+    pattern match {
+      case CS.PatVar(name) =>
+        (DS.PatVar(()), exprSubst.enterBinder(name), typSubst)
+      case CS.PatUnit => (DS.PatUnit, exprSubst, typSubst)
+      case CS.PatTuple(fst, snd) =>
+        val (fstP, eP, tP) = encPat(fst, exprSubst, typSubst)
+        val (sndP, eS, tS) = encPat(snd, eP, tP)
+        (DS.PatTuple(fstP, sndP), eS, tS)
+      case CS.PatConstructor(name, args, body) =>
+        // TODO verify if order is correct here or should be reversed
+        val tP = args.foldLeft(typSubst) {
+          case (subst, arg) => subst.enterBinder(arg)
+        }
+        val (bodyPat, eS, tS) = encPat(body, exprSubst, tP)
+        (DS.PatConstructor(name, args.map(_ => ()), bodyPat), eS, tS)
+    }
+
+  def encSubT(typ: CS.Type, subst: Subst): DS.Type =
+    typ match {
+      case CS.TVar(name) => DS.TVar(subst.deref(name))
+      case CS.TUnit      => DS.TUnit
+      case CS.Tuple(t1, t2) =>
+        DS.Tuple(
+          encSubT(t1, subst),
+          encSubT(t2, subst)
+        )
+      case CS.Fun(arg, res) =>
+        DS.Fun(
+          encSubT(arg, subst),
+          encSubT(res, subst)
+        )
+      case CS.GADT(args, name) =>
+        DS.GADT(args.map(encSubT(_, subst)), name)
+      case CS.Forall(arg, ttyp) =>
+        DS.Forall((), encSubT(ttyp, subst.enterBinder(arg)))
+    }
+
+  implicit class SubstSyntax(substs: Subst) {
+    def lift: Subst =
+      substs.mapValues(_ + 1)
+
+    def enterBinder(name: String): Subst =
+      lift.updated(name, 0)
+
+    def deref(name: String): Int =
+      substs.getOrElse(name, throw UnknownIdentifier(name))
+  }
+}
