tools/src/main/scala/lam2gu/testing/TestExpr.scala
@@ -1,0 +1,17 @@
+package lam2gu.testing
+
+import lam2gu.{LamParser, Lexer}
+
+import scala.io.StdIn
+
+object TestExpr {
+  def main(args: Array[String]): Unit = {
+    while (true) {
+      val ts = StdIn.readLine("Expr:\n")
+      if (ts == null) return
+      println(Lexer(ts))
+      val ex = LamParser.parseExpr(ts)
+      println(ex)
+    }
+  }
+}
