tools/src/main/scala/lam2gu/testing/TestType.scala
@@ -1,0 +1,15 @@
+package lam2gu.testing
+
+import lam2gu.{LamParser, Lexer}
+
+import scala.io.StdIn
+
+object TestType {
+   def main(args: Array[String]): Unit = {
+      while(true) {
+         val ts = StdIn.readLine("Type:\n")
+         val typ = LamParser.parseType(ts)
+         println(typ)
+      }
+   }
+}
