tools/build.sbt
@@ -1,0 +1,18 @@
+name := "LambdaGADT"
+
+version := "0.1"
+
+scalaVersion := "2.12.7"
+
+libraryDependencies += "org.scala-lang.modules" %% "scala-parser-combinators" % "1.1.2"
+
+//libraryDependencies += "org.tpolecat" %% "atto-core"    % "0.7.0"
+//libraryDependencies += "org.tpolecat" %% "atto-refined" % "0.7.0"
+//libraryDependencies += "org.parboiled" %% "parboiled" % "2.1.8"
+
+resolvers += "bintray-djspiewak-maven" at "https://dl.bintray.com/djspiewak/maven"
+
+val ParsebackVersion = "0.3"
+
+//libraryDependencies += "com.codecommit" %% "parseback-core" % ParsebackVersion
+//libraryDependencies += "com.codecommit" %% "parseback-cats" % ParsebackVersion
